define a WP.cmd' in terms of exec, might soon replace WP.cmd
and rules for cmd' whose premises are copied from WP.cmd.
This one is "fs everywhere" (ie list of functions everywhere).
The wp_call rule requires a NoDup, which would be cumbersome to
carry around.

bedrock2/src/bedrock2/WeakestPrecondition.v
@@ -42,6 +42,28 @@ Section WeakestPrecondition.
     Fixpoint expr e := expr_body expr e.
   End WithMemAndLocals.
 
+  Ltac t :=
+    repeat match goal with
+      | |- forall _, _ => progress intros
+      | H: exists _, _ |- _ => destruct H
+      | H: and _ _ |- _ => destruct H
+      | H: eq _ ?y |- _ => subst y
+      | _ => progress cbn in *
+      end; eauto.
+
+  Lemma expr_sound: forall m l e mc post (H : WeakestPrecondition.expr m l e post),
+    exists v mc', Semantics.eval_expr m l e mc = Some (v, mc') /\ post v.
+  Proof.
+    induction e; t.
+    { destruct H. destruct H. eexists. eexists. rewrite H. eauto. }
+    { eapply IHe in H; t. cbv [WeakestPrecondition.load] in H0; t. rewrite H. rewrite H0. eauto. }
+    { eapply IHe in H; t. cbv [WeakestPrecondition.load] in H0; t. rewrite H. rewrite H0. eauto. }
+    { eapply IHe1 in H; t. eapply IHe2 in H0; t. rewrite H, H0; eauto. }
+    { eapply IHe1 in H; t. rewrite H. Tactics.destruct_one_match.
+      { eapply IHe3 in H0; t. }
+      { eapply IHe2 in H0; t. } }
+  Qed.
+
   Section WithF.
     Context {A B} (f: A -> (B -> Prop) -> Prop).
     Definition list_map_body rec (xs : list A) (post : list B -> Prop) : Prop :=
@@ -55,10 +77,348 @@ Section WeakestPrecondition.
     Fixpoint list_map xs := list_map_body list_map xs.
   End WithF.
 
+  Lemma exprs_sound : forall m l args mc P,
+      list_map (expr m l) args P ->
+      exists x mc', Semantics.evaluate_call_args_log m l args mc = Some (x, mc') /\ P x.
+  Proof.
+    induction args; cbn; repeat (subst; t).
+    unfold Semantics.eval_expr in *.
+    eapply expr_sound in H; t; rewrite H.
+    eapply IHargs in H0; t; rewrite H0.
+    eauto.
+  Qed.
+
+  Lemma getmany_sound: forall a l P,
+      list_map (get l) a P -> exists vs, map.getmany_of_list l a = Some vs /\ P vs.
+  Proof.
+    cbv [map.getmany_of_list].
+    induction a; cbn; repeat (subst; t).
+    cbv [WeakestPrecondition.get] in H; t.
+    epose proof (IHa _ _ H0); clear IHa; t.
+    rewrite H. erewrite H1. eexists; split; eauto.
+  Qed.
+
+  Definition dexpr m l e v := expr m l e (eq v).
+  Definition dexprs m l es vs := list_map (expr m l) es (eq vs).
+
+  (* TODO move *)
+  Lemma map__invert_get_of_list{env_ok: map.ok env}: forall ksvs k v,
+      map.get (map.of_list (map := env) ksvs) k = Some v ->
+      List.In k (List.map fst ksvs).
+  Proof.
+    induction ksvs; cbn; intros.
+    - rewrite map.get_empty in H. discriminate H.
+    - destruct a as (k' & v'). rewrite Properties.map.get_put_dec in H.
+      destr.destr (String.eqb k' k).
+      + left. reflexivity.
+      + right. eapply IHksvs. eassumption.
+  Qed.
+
+  Lemma exec_cons_env{env_ok: map.ok env}: forall fname fimpl fs c t m l mc post,
+      ~ List.In fname (List.map fst fs) ->
+      exec (map.of_list fs) c t m l mc post ->
+      exec (map.of_list ((fname, fimpl) :: fs)) c t m l mc post.
+  Proof.
+    induction 2; try solve [econstructor; eauto].
+    econstructor; try eassumption.
+    cbn. rewrite map.get_put_diff. 1: eassumption.
+    intro C. subst fname0.
+    apply H.
+    eapply map__invert_get_of_list.
+    eassumption.
+  Qed.
+
+  Section WithFunctionList1.
+    Context (fs: list (String.string * (list String.string * list String.string * cmd))).
+
+    Inductive cmd' (c : Syntax.cmd) (t : trace) (m : mem) (l : locals)
+      (post : (trace -> mem -> locals -> Prop)) : Prop :=
+    | mk_cmd' (_ : forall mc, exec (map.of_list fs) c t m l mc
+                                (fun t' m' l' mc' => post t' m' l')).
+
+    Lemma invert_cmd': forall c t m l post,
+        cmd' c t m l post ->
+        forall mc, exec (map.of_list fs) c t m l mc (fun t' m' l' mc' => post t' m' l').
+    Proof. intros. inversion H. apply H0. Qed.
+
+    Definition func' '(innames, outnames, c) (t : trace) (m : mem) (args : list word)
+      (post : trace -> mem -> list word -> Prop) :=
+      exists l, map.of_list_zip innames args = Some l /\
+      cmd' c t m l (fun t m l =>
+        list_map (get l) outnames (fun rets =>
+        post t m rets)).
+  End WithFunctionList1.
+
+  Definition call_body' rec (functions : list (String.string * (list String.string * list String.string * cmd.cmd)))
+    (fname : String.string) (t : trace) (m : mem) (args : list word)
+    (post : trace -> mem -> list word -> Prop) : Prop :=
+    match functions with
+    | nil => False
+    | cons (f, decl) functions =>
+        if String.eqb f fname
+        then func' functions decl t m args post
+        else rec functions fname t m args post
+    end.
+  Fixpoint call' functions := call_body' call' functions.
+
+  Section Dedup.
+    Context [A: Type] (aeq: A -> A -> bool).
+
+    (* dedup on (x :: xs) with x having a duplicate in xs discards x, whereas
+     head_prio_dedup keeps x but removes its duplicate from xs *)
+    Fixpoint List__head_prio_dedup (xs : list A) : list A :=
+      match xs with
+      | nil => nil
+      | cons h t => let t' := List__head_prio_dedup t in
+                    cons h (List.removeb aeq h t')
+      end.
+  End Dedup.
+
+  Lemma NoDup_head_prio_dedup[V: Type]: forall (l: list (String.string * V)),
+      List.NoDup (List.map fst (List__head_prio_dedup
+                                  (fun '(f1, _) '(f2, _) => String.eqb f1 f2) l)).
+  Proof.
+    induction l; cbn. 1: constructor.
+    destruct a as (k, v). cbn.
+    constructor.
+    - intro C. eapply List.in_map_iff in C.
+      destruct C as [[k' v'] [E C]]. cbn in E. subst k'.
+      unfold List.removeb in *.
+      eapply List.filter_In in C. apply proj2 in C. rewrite String.eqb_refl in C.
+      discriminate C.
+    -
+  Admitted. (* hopefully holds *)
+
+  Lemma map__get_of_list_filter_diff{env_ok: map.ok env}: forall k k' kvs,
+      k <> k' ->
+      map.get (map.of_list (map := env) kvs) k' =
+      map.get (map.of_list (List.filter
+                      (fun p => negb (let '(kj, _) := p in String.eqb k kj)) kvs)) k'.
+  Proof.
+    induction kvs; cbn; intros. 1: reflexivity.
+    destruct a as (kj & v).
+    rewrite Properties.map.get_put_dec. destr.destr (String.eqb kj k').
+    - destr.destr (String.eqb k k'). 1: contradiction.
+      cbn. rewrite map.get_put_same. reflexivity.
+    - destr.destr (String.eqb k kj); cbn.
+      + eapply IHkvs. assumption.
+      + rewrite map.get_put_diff by congruence. eapply IHkvs. assumption.
+  Qed.
+
+  Lemma map__of_list_ignores_head_prio_dedup{env_ok: map.ok env}: forall ksvs,
+      map.of_list (map := env) ksvs =
+      map.of_list (List__head_prio_dedup (fun '(f1, _) '(f2, _) => String.eqb f1 f2) ksvs).
+  Proof.
+    induction ksvs; cbn. 1: reflexivity.
+    destruct a as (k & v).
+    eapply map.map_ext.
+    intros k'. rewrite? Properties.map.get_put_dec. destr.destr (String.eqb k k').
+    1: reflexivity.
+    rewrite IHksvs.
+    unfold List.removeb.
+    remember (List__head_prio_dedup (fun '(f1, _) '(f2, _) => String.eqb f1 f2) ksvs) as L.
+    apply map__get_of_list_filter_diff. assumption.
+  Qed.
+
+  Lemma call'_ignores_head_prio_dedup_otherdirection{env_ok: map.ok env}:
+    forall fs fname t m args post,
+      call' (List__head_prio_dedup (fun '(f1, _) '(f2, _) => String.eqb f1 f2) fs)
+            fname t m args post ->
+      call' fs fname t m args post.
+  Proof.
+    induction fs; cbn; intros. 1: assumption.
+    destruct a as (f, decl). destr.destr (String.eqb f fname).
+    - unfold func' in *. destruct decl as ((argnames, retnames), body).
+      destruct H as (l & Hl & Hbody). exists l. split. 1: exact Hl.
+      inversion Hbody. constructor. intro mc. specialize (H mc).
+      rewrite map__of_list_ignores_head_prio_dedup in H.
+  Abort.
+
+  Lemma call'_ignores_head_prio_dedup{env_ok: map.ok env}:
+    forall fs fname t m args post,
+      call' fs fname t m args post ->
+      call' (List__head_prio_dedup (fun '(f1, _) '(f2, _) => String.eqb f1 f2) fs)
+            fname t m args post.
+  Proof.
+    induction fs; cbn; intros. 1: assumption.
+    destruct a as (f, decl). destr.destr (String.eqb f fname).
+    - unfold func' in *. destruct decl as ((argnames, retnames), body).
+      destruct H as (l & Hl & Hbody). exists l. split. 1: exact Hl.
+      constructor. intro mc. eapply invert_cmd' in Hbody.
+      rewrite map__of_list_ignores_head_prio_dedup in Hbody.
+  Admitted. (* TODO probably DOES NOT HOLD because recursive call of call' is made
+               on smaller env with current function removed *)
+
+  Section WithFunctionList2.
+    Implicit Type post : trace -> mem -> locals -> Prop.
+    Context (fs: list (String.string * (list String.string * list String.string * cmd))).
+
+    Notation cmd' := (cmd' fs).
+
+    Ltac step :=
+      match reverse goal with
+      | H: _ /\ _ |- _ => destruct H
+      | H: exists x, _ |- _ => let n := fresh x in destruct H as [n H]
+      | |- _ => progress unfold dlet, dexpr, store in *
+      | H: cmd' _ _ _ _ _ |- _ => pose proof (invert_cmd' _ _ _ _ _ _ H); clear H
+      | |- _ => constructor
+      | |- _ => assumption
+      | H: forall _: MetricLogging.MetricLog, _ |- _ => apply H
+      | |- _ => progress intros
+      | |- _ => progress subst
+      (* creates an evar for metrics, therefore needs to be applied from top to bottom,
+         so we need `match reverse` instead of `match` *)
+      | H: expr _ _ _ _ |- _ => eapply expr_sound in H
+      | |- _ => solve [econstructor; eauto]
+      end.
+    Ltac tac := repeat step.
+
+    Lemma wp_skip: forall t m l post, post t m l -> cmd' cmd.skip t m l post.
+    Proof. tac. Qed.
+
+    Lemma wp_set: forall x ev t m l post,
+        (exists v, dexpr m l ev v /\
+        dlet! l := map.put l x v in
+        post t m l) ->
+        cmd' (cmd.set x ev) t m l post.
+    Proof. tac. Qed.
+
+    Lemma wp_unset: forall x t m l post,
+        (dlet! l := map.remove l x in
+         post t m l) ->
+        cmd' (cmd.unset x) t m l post.
+    Proof. tac. Qed.
+
+    Lemma wp_store: forall sz ea ev t m l post,
+       (exists a, dexpr m l ea a /\
+        exists v, dexpr m l ev v /\
+        store sz m a v (fun m =>
+        post t m l)) ->
+       cmd' (cmd.store sz ea ev) t m l post.
+    Proof. tac. Qed.
+
+    Lemma wp_stackalloc: forall x n c t m l post,
+        (Z.modulo n (bytes_per_word width) = 0 /\
+        forall a mStack mCombined,
+          anybytes a n mStack -> map.split mCombined m mStack ->
+          dlet! l := map.put l x a in
+          cmd' c t mCombined l (fun t' mCombined' l' =>
+          exists m' mStack',
+          anybytes a n mStack' /\ map.split mCombined' m' mStack' /\
+          post t' m' l')) ->
+          cmd' (cmd.stackalloc x n c) t m l post.
+    Proof. tac. specialize H0 with (1 := H1) (2 := H2). tac. Qed.
+
+    Lemma wp_cond: forall br ct cf t m l post,
+        (exists v, dexpr m l br v /\
+        (word.unsigned v <> 0%Z -> cmd' ct t m l post) /\
+        (word.unsigned v = 0%Z -> cmd' cf t m l post)) ->
+        cmd' (cmd.cond br ct cf) t m l post.
+    Proof.
+      tac. destr.destr (Z.eqb (word.unsigned v0) 0).
+      - specialize H1 with (1 := E). tac.
+      - specialize H0 with (1 := E). tac.
+    Qed.
+
+    Lemma wp_seq: forall c1 c2 t m l post,
+        cmd' c1 t m l (fun t m l => cmd' c2 t m l post) ->
+        cmd' (cmd.seq c1 c2) t m l post.
+    Proof.
+      tac. eapply exec.weaken.
+      { econstructor. 1: eapply H0. tac. }
+      tac.
+    Qed.
+
+    Lemma wp_while: forall e c t m l post,
+       (exists measure (lt:measure->measure->Prop) (inv:measure->trace->mem->locals->Prop),
+        Coq.Init.Wf.well_founded lt /\
+        (exists v, inv v t m l) /\
+        (forall v t m l, inv v t m l ->
+          exists b, dexpr m l e b /\
+          (word.unsigned b <> 0%Z -> cmd' c t m l (fun t' m l =>
+            exists v', inv v' t' m l /\ lt v' v)) /\
+          (word.unsigned b = 0%Z -> post t m l))) ->
+       cmd' (cmd.while e c) t m l post.
+    Proof.
+      intros. destruct H as (measure & lt & inv & Hwf & HInit & Hbody).
+      destruct HInit as (v0 & HInit).
+      econstructor. intros.
+      revert t m l mc HInit. pattern v0. revert v0.
+      eapply (well_founded_ind Hwf). intros.
+      specialize Hbody with (1 := HInit). destruct Hbody as (b & Hb & Ht & Hf).
+      eapply expr_sound in Hb. destruct Hb as (b' & mc' & Hb & ?). subst b'.
+      destr.destr (Z.eqb (word.unsigned b) 0).
+      - specialize Hf with (1 := E). eapply exec.while_false; eassumption.
+      - specialize Ht with (1 := E). inversion Ht. clear Ht.
+        eapply exec.while_true; eauto.
+        cbv beta. intros * (v' & HInv & HLt). eauto.
+    Qed.
+
+    Lemma wp_call0{env_ok: map.ok env}
+      (Hnd : List.NoDup (List.map fst fs)): (* <--------- *)
+      forall binds fname arges t m l post,
+       (exists args, dexprs m l arges args /\
+        call' fs fname t m args (fun t m rets =>
+          exists l', map.putmany_of_list_zip binds rets l = Some l' /\
+          post t m l')) ->
+       cmd' (cmd.call binds fname arges) t m l post.
+    Proof.
+      tac.
+      unfold dexprs in *.
+      eapply exprs_sound in H. destruct H as (argvs & mc' & HEv & ?). subst argvs.
+      unfold call' in *.
+      revert fname H0. induction fs; intros.
+      - cbn in H0. contradiction.
+      - rename l0 into fs0.
+        destruct a as (fnameHere & ((argnames & retnames) & fbody)).
+        inversion Hnd. subst.
+        cbn in H0.
+        destr.destr (String.eqb fnameHere fname).
+        + destruct H0 as (l1 & Hl1 & Hbody).
+          inversion Hbody. clear Hbody. rename H into Hbody.
+          eapply exec.call.
+          * cbn. rewrite map.get_put_same. reflexivity.
+          * eassumption.
+          * eassumption.
+          * eapply exec_cons_env. 1: assumption. apply Hbody.
+          * cbv beta. intros. eapply getmany_sound. assumption.
+        + eapply exec_cons_env. 1: assumption.
+          eapply IHl0; assumption.
+    Qed.
+
+    Lemma wp_interact: forall binds action arges t m l post,
+       (exists args, dexprs m l arges args /\
+        exists mKeep mGive, map.split m mKeep mGive /\
+        ext_spec t mGive action args (fun mReceive rets =>
+          exists l', map.putmany_of_list_zip binds rets l = Some l' /\
+          forall m', map.split m' mKeep mReceive ->
+          post (cons ((mGive, action, args), (mReceive, rets)) t) m' l')) ->
+       cmd' (cmd.interact binds action arges) t m l post.
+    Proof.
+      tac.
+      eapply exprs_sound in H. destruct H as (argvs & mc' & HEv & ?). subst argvs.
+      tac.
+    Qed.
+  End WithFunctionList2.
+
+  (* without NoDup assumption, but probably doesn't hold *)
+  Lemma wp_call{env_ok: map.ok env}: forall fs binds fname arges t m l post,
+      (exists args, dexprs m l arges args /\
+       call' fs fname t m args (fun t m rets =>
+       exists l', map.putmany_of_list_zip binds rets l = Some l' /\
+       post t m l')) ->
+      cmd' fs (cmd.call binds fname arges) t m l post.
+  Proof.
+    intros. destruct H as (args & Hargs & H).
+    constructor. rewrite map__of_list_ignores_head_prio_dedup. eapply invert_cmd'.
+    eapply (wp_call0 _ (env_ok := env_ok)).
+    1: eapply NoDup_head_prio_dedup.
+    eexists. split. 1: eassumption.
+    eapply call'_ignores_head_prio_dedup. assumption.
+  Qed.
+
   Section WithFunctions.
     Context (call : String.string -> trace -> mem -> list word -> (trace -> mem -> list word -> Prop) -> Prop).
-    Definition dexpr m l e v := expr m l e (eq v).
-    Definition dexprs m l es vs := list_map (expr m l) es (eq vs).
     Definition cmd_body (rec:_->_->_->_->_->Prop) (c : cmd) (t : trace) (m : mem) (l : locals)
              (post : trace -> mem -> locals -> Prop) : Prop :=
       (* give value of each pure expression when stating its subproof *)
